fix npbc_full (others not fixed yet)

examples/pseudo_bool/array/npbc_arrayProgScript.sml
@@ -2835,7 +2835,6 @@ End
 
 val res = translate change_obj_update_def;
 
-(* TODO: update below here *)
 val check_cstep_arr = process_topdecs`
   fun check_cstep_arr lno cstep fml inds pc =
   case cstep of
@@ -3508,7 +3507,7 @@ Proof
   fs[LIST_REL_EL_EQN]
 QED
 
-val _ = register_type ``:houtput``
+val _ = register_type ``:output``
 
 Definition eq_none_def:
   eq_none (bnd: int option) =
@@ -3533,24 +3532,24 @@ End
 val res = translate eq_opt_chk_def;
 
 (* written in a funny way to make CF easier *)
-val check_houtput_arr = process_topdecs`
-  fun check_houtput_arr fml inds
-    obj bound dbound chk houtput =
-  case houtput of
-    Hnooutput => True
-  | Hderivable fml' =>
+val check_output_arr = process_topdecs`
+  fun check_output_arr fml inds
+    obj bound dbound chk fml' obj' output =
+  case output of
+    Nooutput => True
+  | Derivable =>
     let val cls = map_snd (core_fmlls_arr fml inds) in
     if eq_none dbound then fml_include_arr cls fml'
     else False
     end
-  | Hequisatisfiable fml' =>
+  | Equisatisfiable =>
     let val cls = map_snd (core_fmlls_arr fml inds) in
     if eq_sat_chk bound dbound chk then
       fml_include_arr cls fml' andalso
       fml_include_arr fml' cls
     else False
     end
-  | Hequioptimal fml' obj' =>
+  | Equioptimal =>
     let val cls = map_snd (core_fmlls_arr fml inds) in
       if eq_opt_chk bound dbound chk obj obj' then
         fml_include_arr cls fml' andalso
@@ -3558,31 +3557,34 @@ val check_houtput_arr = process_topdecs`
       else False
     end` |> append_prog;
 
-val NPBC_HOUTPUT_TYPE_def = theorem"NPBC_HOUTPUT_TYPE_def";
+val PBC_OUTPUT_TYPE_def = theorem"PBC_OUTPUT_TYPE_def";
 
-Theorem check_houtput_arr_spec:
+Theorem check_output_arr_spec:
   (LIST_TYPE NUM) inds indsv ∧
   obj_TYPE obj objv ∧
   OPTION_TYPE INT bound boundv ∧
   OPTION_TYPE INT dbound dboundv ∧
   BOOL chk chkv ∧
-  NPBC_HOUTPUT_TYPE houtput houtputv ∧
+  PBC_OUTPUT_TYPE output outputv ∧
+  LIST_TYPE constraint_TYPE fmlt fmltv ∧
+  obj_TYPE objt objtv ∧
   LIST_REL (OPTION_TYPE bconstraint_TYPE) fmlls fmllsv
   ⇒
   app (p : 'ffi ffi_proj)
-    ^(fetch_v "check_houtput_arr" (get_ml_prog_state()))
-    [fmlv; indsv; objv; boundv; dboundv; chkv; houtputv]
+    ^(fetch_v "check_output_arr" (get_ml_prog_state()))
+    [fmlv; indsv; objv; boundv; dboundv; chkv;
+      fmltv; objtv; outputv]
     (ARRAY fmlv fmllsv)
     (POSTv v.
         ARRAY fmlv fmllsv *
         &(
-        BOOL (check_houtput_list fmlls inds obj
-          bound dbound chk houtput) v))
+        BOOL (check_output_list fmlls inds obj
+          bound dbound chk fmlt objt output) v))
 Proof
   rw[]>>
-  xcf"check_houtput_arr"(get_ml_prog_state ())>>
-  Cases_on`houtput`>>
-  fs[npbc_listTheory.check_houtput_list_def,NPBC_HOUTPUT_TYPE_def]>>
+  xcf"check_output_arr"(get_ml_prog_state ())>>
+  Cases_on`output`>>
+  fs[npbc_listTheory.check_output_list_def,PBC_OUTPUT_TYPE_def]>>
   xmatch
   >-
     (xcon>>xsimpl)
